chore: add Bool into Reflect as well

SSA/Experimental/Bits/Fast/Defs.lean
@@ -107,7 +107,17 @@ def BTerm.evalFin (t : BTerm) (vars : Fin (arity t) → BitStream) : BitStream :
 /--
 If they are equal so far, then `t1 ^^^ t2`.scanOr will be 0.
 -/
-def Predicate.evalEq (t₁ t₂ : BitStream) : BitStream := (t₁ ^^^ t₂).concat false |>.scanOr
+def Predicate.evalBitstreamEq (t₁ t₂ : BitStream) : BitStream := (t₁ ^^^ t₂) |>.scanOr
+
+/--
+If they are equal so far, then `t1 ^^^ t2`.scanOr will be 0.
+-/
+def Predicate.evalBitstreamNeq (t₁ t₂ : BitStream) : BitStream := (t₁.nxor t₂) |>.scanAnd
+
+/--
+If they are equal so far, then `t1 ^^^ t2`.scanOr will be 0.
+-/
+def Predicate.evalBVEq (t₁ t₂ : BitStream) : BitStream := (t₁ ^^^ t₂).concat false |>.scanOr
 /--
 If they have been equal so far, then `BitStream.nxor t₁ t₂`.scanAnd will be 1.
 Start by assuming that they are not (not equal) i.e. that they are equal, and the
@@ -115,7 +125,7 @@ Start by assuming that they are not (not equal) i.e. that they are equal, and th
 If their values ever differ, then we know that we will have `a[i] == b[i]` to be `false`.
 From this point onward, they will always disagree, and thus the predicate should become `0`.
 -/
-def Predicate.evalNeq (t₁ t₂ : BitStream) : BitStream := (t₁.nxor t₂).concat true |>.scanAnd
+def Predicate.evalBVNeq (t₁ t₂ : BitStream) : BitStream := (t₁.nxor t₂).concat true |>.scanAnd
 
 /-
 If they have been `0` so far, then `t1 &&& t2 |>.scanOr` will be `1`.
@@ -180,23 +190,25 @@ def Predicate.eval (p : Predicate) (vars : List BitStream) : BitStream :=
   | .width .ge n => BitStream.falseIffGe n
   | lor p q => Predicate.evalLor (p.eval vars) (q.eval vars)
   | land p q => Predicate.evalLand (p.eval vars) (q.eval vars)
-  | boolBinary .eq t₁ t₂ => Predicate.evalEq (t₁.eval vars) (t₂.eval vars)
-  | boolBinary .neq t₁ t₂ => Predicate.evalNeq (t₁.eval vars) (t₂.eval vars)
-  | binary .eq t₁ t₂ => Predicate.evalEq (t₁.eval vars) (t₂.eval vars)
+  /- boolean operations. -/
+  | boolBinary .eq t₁ t₂ => Predicate.evalBitstreamEq (t₁.eval vars) (t₂.eval vars)
+  | boolBinary .neq t₁ t₂ => Predicate.evalBitstreamNeq (t₁.eval vars) (t₂.eval vars)
+  /- bitstream operations. -/
+  | binary .eq t₁ t₂ => Predicate.evalBVEq (t₁.eval vars) (t₂.eval vars)
   /-
   If it is ever not equal, then we want to stay not equals for ever.
   So, if the 'a = b' returns 'false' at some index 'i', we will stay false
   for all indexes '≥ i'.
   -/
-  | binary .neq t1 t2 => Predicate.evalNeq (t1.eval vars) (t2.eval vars)
+  | binary .neq t1 t2 => Predicate.evalBVNeq (t1.eval vars) (t2.eval vars)
   | binary .ult t₁ t₂ => Predicate.evalUlt (t₁.eval vars) (t₂.eval vars)
   | binary .ule t₁ t₂ =>
      Predicate.evalLor
-       (Predicate.evalEq (t₁.eval vars) (t₂.eval vars))
+       (Predicate.evalBVEq (t₁.eval vars) (t₂.eval vars))
        (Predicate.evalUlt (t₁.eval vars) (t₂.eval vars))
   | binary .slt t₁ t₂ => Predicate.evalSlt (t₁.eval vars) (t₂.eval vars)
   | binary .sle t₁ t₂ => Predicate.evalLor
-       (Predicate.evalEq (t₁.eval vars) (t₂.eval vars))
+       (Predicate.evalBVEq (t₁.eval vars) (t₂.eval vars))
        (Predicate.evalSlt (t₁.eval vars) (t₂.eval vars))
 
 @[simp]
@@ -231,19 +243,20 @@ match p with
 | .boolBinary .eq t₁ t₂ =>
     let x₁ := t₁.evalFin (fun i => vars (Fin.castLE (by simp [arity]) i))
     let x₂ := t₂.evalFin (fun i => vars (Fin.castLE (by simp [arity]) i))
-    x₁ ^^^ x₂
+    Predicate.evalBitstreamEq x₁ x₂
 | .boolBinary .neq t₁ t₂ =>
     let x₁ := t₁.evalFin (fun i => vars (Fin.castLE (by simp [arity]) i))
     let x₂ := t₂.evalFin (fun i => vars (Fin.castLE (by simp [arity]) i))
-    ~~~ (x₁ ^^^ x₂)
+    Predicate.evalBitstreamNeq x₁ x₂
+    -- ~~~ (x₁ ^^^ x₂)
 | .binary .eq t₁ t₂ =>
     let x₁ := t₁.evalFin (fun i => vars (Fin.castLE (by simp [arity]) i))
     let x₂ := t₂.evalFin (fun i => vars (Fin.castLE (by simp [arity]) i))
-    Predicate.evalEq x₁ x₂
+    Predicate.evalBVEq x₁ x₂
 | .binary .neq t₁ t₂  =>
     let x₁ := t₁.evalFin (fun i => vars (Fin.castLE (by simp [arity]) i))
     let x₂ := t₂.evalFin (fun i => vars (Fin.castLE (by simp [arity]) i))
-    Predicate.evalNeq x₁ x₂
+    Predicate.evalBVNeq x₁ x₂
 | .land p q =>
   -- if both `p` and `q` are logically true (i.e. the predicate is `false`),
   -- only then should we return a `false`.
@@ -262,7 +275,7 @@ match p with
 | .binary .sle p q =>
   let x₁ := p.evalFin (fun i => vars (Fin.castLE (by simp [arity]) i))
   let x₂ := q.evalFin (fun i => vars (Fin.castLE (by simp [arity]) i))
-  Predicate.evalLor (Predicate.evalSlt x₁ x₂) (Predicate.evalEq x₁ x₂)
+  Predicate.evalLor (Predicate.evalSlt x₁ x₂) (Predicate.evalBVEq x₁ x₂)
 | .binary .ult p q =>
   let x₁ := p.evalFin (fun i => vars (Fin.castLE (by simp [arity]) i))
   let x₂ := q.evalFin (fun i => vars (Fin.castLE (by simp [arity]) i))
@@ -270,4 +283,4 @@ match p with
 | .binary .ule p q =>
   let x₁ := p.evalFin (fun i => vars (Fin.castLE (by simp [arity]) i))
   let x₂ := q.evalFin (fun i => vars (Fin.castLE (by simp [arity]) i))
-  Predicate.evalLor (Predicate.evalUlt x₁ x₂) (Predicate.evalEq x₁ x₂)
+  Predicate.evalLor (Predicate.evalUlt x₁ x₂) (Predicate.evalBVEq x₁ x₂)
