SSA/Experimental/Bits/Fast/Reflect.lean
@@ -302,12 +302,12 @@ def Predicate.cost (p : Predicate) : Nat :=
 
 
 /-
-if 'evalEq' evaluates to 'false', then indeed the denotations of the terms are equal.
+if 'evalBVEq' evaluates to 'false', then indeed the denotations of the terms are equal.
 -/
-theorem Predicate.evalEq_denote_false_iff {w : Nat} (a b : Term) (vars : List (BitVec w)) :
-    evalEq (a.eval (List.map BitStream.ofBitVec vars)) (b.eval (List.map BitStream.ofBitVec vars)) w = false ↔
+theorem Predicate.evalBVEq_denote_false_iff {w : Nat} (a b : Term) (vars : List (BitVec w)) :
+    evalBVEq (a.eval (List.map BitStream.ofBitVec vars)) (b.eval (List.map BitStream.ofBitVec vars)) w = false ↔
     Term.denote w a vars = Term.denote w b vars := by
-  simp [evalEq]
+  simp [evalBVEq]
   constructor
   · intros h
     /- Dear god, this proof is ugly. -/
@@ -326,13 +326,13 @@ theorem Predicate.evalEq_denote_false_iff {w : Nat} (a b : Term) (vars : List (B
     · simp
       rw [Term.eval_eq_denote_apply a (by omega), Term.eval_eq_denote_apply b (by omega), h]
 
-/-- evalEq is true iff evalNeq is false -/
-theorem Predicate.evalEq_iff_not_evalNeq (a b : BitStream) :
-    ∀ (w : Nat), evalEq a b w ↔ ¬ (evalNeq a b w) := by
+/-- evalBVEq is true iff evalBVNeq is false -/
+theorem Predicate.evalBVEq_iff_not_evalNeq (a b : BitStream) :
+    ∀ (w : Nat), evalBVEq a b w ↔ ¬ (evalBVNeq a b w) := by
   intros w
   rcases w with rfl | w
-  · simp [evalEq, evalNeq]
-  · simp [evalEq, evalNeq]
+  · simp [evalBVEq, evalBVNeq]
+  · simp [evalBVEq, evalBVNeq]
     by_cases hab : a w = b w
     · simp [hab]
       by_cases heq : (BitStream.concat false (a ^^^ b)).scanOr w
@@ -361,29 +361,29 @@ theorem Predicate.evalEq_iff_not_evalNeq (a b : BitStream) :
 
 /-- 'evalNeq' correctly witnesses when terms are disequal -/
 theorem Predicate.evalNeq_denote {w : Nat} (a b : Term) (vars : List (BitVec w)) :
-    evalNeq (a.eval (List.map BitStream.ofBitVec vars)) (b.eval (List.map BitStream.ofBitVec vars)) w = false ↔
+    evalBVNeq (a.eval (List.map BitStream.ofBitVec vars)) (b.eval (List.map BitStream.ofBitVec vars)) w = false ↔
     Term.denote w a vars ≠ Term.denote w b vars := by
   constructor
   · intros h
-    apply Predicate.evalEq_denote_false_iff .. |>.not.mp
+    apply Predicate.evalBVEq_denote_false_iff .. |>.not.mp
     simp only [Bool.not_eq_false]
-    have := Predicate.evalEq_iff_not_evalNeq
+    have := Predicate.evalBVEq_iff_not_evalNeq
       (a.eval (List.map BitStream.ofBitVec vars))
       (b.eval (List.map BitStream.ofBitVec vars))
     apply this .. |>.mpr
     simp [h]
   · intros h
-    have this' := Predicate.evalEq_denote_false_iff .. |>.not.mpr h
+    have this' := Predicate.evalBVEq_denote_false_iff .. |>.not.mpr h
     simp at this'
-    have := Predicate.evalEq_iff_not_evalNeq
+    have := Predicate.evalBVEq_iff_not_evalNeq
       (a.eval (List.map BitStream.ofBitVec vars))
       (b.eval (List.map BitStream.ofBitVec vars)) w |>.mp this'
     simpa using this
 
-theorem Predicate.evalEq_denote_true_iff {w : Nat} (a b : Term) (vars : List (BitVec w)) :
-    evalEq (a.eval (List.map BitStream.ofBitVec vars)) (b.eval (List.map BitStream.ofBitVec vars)) w = true ↔
+theorem Predicate.evalBVEq_denote_true_iff {w : Nat} (a b : Term) (vars : List (BitVec w)) :
+    evalBVEq (a.eval (List.map BitStream.ofBitVec vars)) (b.eval (List.map BitStream.ofBitVec vars)) w = true ↔
     Term.denote w a vars ≠ Term.denote w b vars := by
-  rw [Predicate.evalEq_iff_not_evalNeq]
+  rw [Predicate.evalBVEq_iff_not_evalNeq]
   simp [evalNeq_denote]
 
 
@@ -537,7 +537,7 @@ theorem Predicate.eval_eq_denote (w : Nat) (p : Predicate) (vars : List (BitVec 
   case width wp n => cases wp <;> simp [eval, denote]
   case binary p a b =>
     cases p with
-    | eq => simp [eval, denote]; apply evalEq_denote_false_iff
+    | eq => simp [eval, denote]; apply evalBVEq_denote_false_iff
     | neq => simp [eval, denote]; apply evalNeq_denote
     | ult =>
       simp [eval, denote]
@@ -563,13 +563,13 @@ theorem Predicate.eval_eq_denote (w : Nat) (p : Predicate) (vars : List (BitVec 
       rw [BitVec.ForLean.ule_iff_ult_or_eq' (Term.denote w a vars) (Term.denote w b vars)]
       by_cases heq : Term.denote w a vars = Term.denote w b vars
       · rw [heq]
-        simp [evalEq_denote_false_iff a b vars |>.mpr heq]
+        simp [evalBVEq_denote_false_iff a b vars |>.mpr heq]
       · simp [heq]
         by_cases hlt : Term.denote w a vars < Term.denote w b vars
         · simp [hlt]
           simp [evalUlt_denote_false_iff a b vars |>.mpr hlt]
         · simp [hlt]
-          have := evalEq_denote_false_iff a b vars |>.not |>.mpr heq
+          have := evalBVEq_denote_false_iff a b vars |>.not |>.mpr heq
           simp only [this, true_and]
           have := evalUlt_denote_false_iff a b vars |>.not |>.mpr hlt
           simp only [this]
@@ -580,12 +580,12 @@ theorem Predicate.eval_eq_denote (w : Nat) (p : Predicate) (vars : List (BitVec 
       rcases hSle : Term.denote w a vars ≤ₛ Term.denote w b vars
       · simp [hSle] at h ⊢
         obtain ⟨h₁, h₂⟩ := h
-        simp [evalEq_denote_true_iff .. |>.mpr h₁]
+        simp [evalBVEq_denote_true_iff .. |>.mpr h₁]
         rw [evalSlt_denote_true_iff .. |>.mpr]
         simp [h₂]
       · simp [hSle] at h ⊢
         intros hEq
-        simp [evalEq_denote_true_iff .. |>.mp hEq] at h
+        simp [evalBVEq_denote_true_iff .. |>.mp hEq] at h
         apply evalSlt_denote_false_iff .. |>.mpr h
   case land p q hp hq => simp [eval, denote, hp, hq, evalLand]
   case lor p q hp hq =>
@@ -607,6 +607,13 @@ theorem Predicate.eval_eq_denote (w : Nat) (p : Predicate) (vars : List (BitVec 
         simp [this]
       · have := hq .. |>.mpr hq'
         simp [this]
+
+  case boolBinary p a b =>
+    cases p with
+    | eq =>
+      simp [eval, denote]; sorry
+    | neq =>
+      simp [eval, denote]; sorry
 
 -- /-- info: 'Predicate.eval_eq_denote' depends on axioms: [propext, Classical.choice, Quot.sound] -/
 -- #guard_msgs in #print axioms Predicate.eval_eq_denote
